src/HarvardMachine.v
@@ -1,0 +1,84 @@
+Require Import Coq.ZArith.BinInt.
+Require Import bbv.WordScope.
+Require Import bbv.DepEqNat.
+Require Import riscv.util.NameWithEq.
+Require Import riscv.RiscvBitWidths.
+Require Import riscv.util.Monads.
+Require Import riscv.Decode.
+Require Import riscv.Memory. (* should go before Program because both define loadByte etc *)
+Require Import riscv.Program.
+Require Import riscv.Execute.
+Require Import riscv.util.PowerFunc.
+Require Import riscv.Utility.
+Require Import Coq.Lists.List. Import ListNotations.
+Require Import riscv.Minimal.
+Require Import riscv.PseudoInstructions.
+Require Import riscv.InstructionCoercions.
+Require Import riscv.FunctionMemory.
+
+Section Riscv.
+
+  Context {B: RiscvBitWidths}.
+
+  Context {MW: MachineWidth (word wXLEN)}.
+
+  Definition InstructionMem := word wXLEN -> Instruction.
+  
+  Record HarvardMachine := mkHarvardMachine {
+    machine: @RiscvMachine _ (mem wXLEN);
+    instructionMem: InstructionMem;
+  }.
+
+  Definition with_machine m ml := mkHarvardMachine m ml.(instructionMem).
+  Definition with_instructionMem l ml := mkHarvardMachine ml.(machine) l.  
+
+  Definition liftL0{B: Type}(f: OState RiscvMachine B):  OState HarvardMachine B :=
+    fun s => let (ob, ma) := f s.(machine) in (ob, with_machine ma s).
+
+  Definition liftL1{A B: Type}(f: A -> OState RiscvMachine B): A -> OState HarvardMachine B :=
+    fun a s => let (ob, ma) := f a s.(machine) in (ob, with_machine ma s).
+
+  Definition liftL2{A1 A2 B: Type}(f: A1 -> A2 -> OState RiscvMachine B):
+    A1 -> A2 -> OState HarvardMachine B :=
+    fun a1 a2 s => let (ob, ma) := f a1 a2 s.(machine) in (ob, with_machine ma s).
+                                           
+  Instance IsHarvardMachine: RiscvProgram (OState HarvardMachine) (word wXLEN) :=  {|
+      getRegister := liftL1 getRegister;
+      setRegister := liftL2 setRegister;
+      getPC := liftL0 getPC;
+      setPC := liftL1 setPC;
+      loadByte   := liftL1 loadByte;
+      loadHalf   := liftL1 loadHalf;
+      loadWord   := liftL1 loadWord;
+      loadDouble := liftL1 loadDouble;
+      storeByte   := liftL2 storeByte;
+      storeHalf   := liftL2 storeHalf;
+      storeWord   := liftL2 storeWord;
+      storeDouble := liftL2 storeDouble;
+      step := liftL0 step;
+      getCSRField_MTVecBase := liftL0 getCSRField_MTVecBase;
+      endCycle A := Return None;
+  |}.
+
+  Definition putProgram(prog: list (word 32))(ma: HarvardMachine): HarvardMachine :=
+    with_machine (putProgram prog ma.(machine)) ma.
+
+  Definition loadInst(addr: word wXLEN): OState HarvardMachine Instruction :=
+    im <- gets instructionMem;
+    Return (im addr).
+
+  (* assumes generic translate and raiseException functions *)
+  Context {RVS: RiscvState (OState HarvardMachine) (word wXLEN)}.
+  
+  Definition run1: OState HarvardMachine unit :=
+    pc <- getPC;
+    inst <- loadInst pc;
+    execute inst;;
+    step.
+
+  Definition run: nat -> OState HarvardMachine unit :=
+    fun n => power_func (fun m => run1 ;; m) n (Return tt).
+  
+End Riscv.
+
+Existing Instance IsHarvardMachine. (* needed because it was defined inside a Section *)
